Work in progress on rep relation

theories/Glue/rep.v
@@ -22,8 +22,10 @@
   [ ] polymorphic types like [option]
   [ ] multi-polymorphic types like [pair]
   [ ] recursive and polymorphic types like [list]
-  [ ] recursive and dependent types like [vector]
-  [ ] types of sort Prop like [and] or [le]
+  [ ] recursive and dependent types like [fin]
+  [ ] recursive, polymorphic and dependent types like [vector]
+  [ ] types of sort Prop like [True], [and] or [le]
+  [ ] types that use functions in its definition
 
   Game plan:
   * Take a type constructor (in Coq, not reified) as an input.
@@ -36,6 +38,12 @@
       quantify over all parameters and indices.
   * If a block is missing any instance,
     define type class instances for each type in the block.
+
+  Caveats:
+  * If a type is of sort [Prop], the representation of its values is
+    the same as [unit] for all vallues.
+  * Parameters are not included in the memory representation,
+    indices are.
 *)
 Require Import Coq.ZArith.ZArith
                Coq.Program.Basics
@@ -53,7 +61,23 @@ Require Import MetaCoq.Template.All.
 
 Require Import glue_utils.
 
+(* Warning: MetaCoq doesn't use the Monad notation from ExtLib,
+  therefore don't expect ExtLib functions to work with TemplateMonad. *)
+Import monad_utils.MonadNotation
+       ListNotations
+       MetaCoqNotations.
+
 Require CertiCoq.L6.Prototype.
+(* Alias to distinguish terms that are NOT in de Bruijn notation. *)
+Definition named_term : Type := term.
+(* Alias for terms that do not contain references to local variables,
+   therefore can be used in either [term]s in de Bruijn notation
+   and [named_term]s in named notation. *)
+Definition global_term : Type := term.
+(* Alias to denote that a function works with
+   either [term], [named_term] or [global_term]. *)
+Definition any_term : Type := term.
+
 Module DB.
   (* Uses code written by John Li.
      We should eventually consider making a MetaCoq_utils module. *)
@@ -67,36 +91,35 @@ Module DB.
 
   (* Takes a named representation, which we hack by using names starting with $,
      and converts it into the de Bruijn representation. *)
-  Definition deBruijn (t : term) : TemplateMonad term :=
+  Definition deBruijn (t : named_term) : TemplateMonad term :=
     runGM (indices_of [] t).
 
   (* Example usage for deBruijn:
 
-     MetaCoq Run (t <- DB.deBruijn <% fun (x : bool) => x %> ;;
+     MetaCoq Run (t <- DB.deBruijn
+                          (tLambda (nNamed "$x") <% bool %> (tVar "$x")) ;;
+                  t' <- tmUnquoteTyped (bool -> bool) t ;;
                   tmPrint t).
   *)
 
   (* Takes a de Bruijn representation and adds $ to local variables,
      and changes [tRel]s to [tVar]s referring to those variabstarting with $. *)
-  Definition undeBruijn (initial : list ident) (t : term) : TemplateMonad term :=
+  Definition undeBruijn (initial : list ident)
+                        (t : term) : TemplateMonad named_term :=
     runGM (named_of initial t).
 
   (* Example usage for undeBruijn:
 
-     MetaCoq Run (t <- DB.undeBruijn nil (tLambda (nNamed "$x") <% bool %> (tVar "$x")) ;;
-                  t' <- tmUnquoteTyped (bool -> bool) t ;;
+     MetaCoq Run (t <- DB.undeBruijn nil <% fun (x : bool) => x %> ;;
                   tmPrint t).
   *)
 End DB.
 
-(* Warning: MetaCoq doesn't use the Monad notation from ExtLib,
-  therefore don't expect ExtLib functions to work with TemplateMonad. *)
-Import monad_utils.MonadNotation
-       ListNotations
-       MetaCoqNotations.
-
 Notation "f >=> g" := (fun x => (f x) >>= g)
                       (at level 51, right associativity) : monad_scope.
+Notation "f <$> x" := (x' <- x%monad ;; ret (f x'))
+                      (at level 52, right associativity) : monad_scope.
+
 
 Variables (graph : Type) (mtype : Type).
 
@@ -109,59 +132,20 @@ Variable fitting_index : graph -> mtype -> cRep -> list mtype -> Prop.
 Class Rep (A : Type) : Type :=
   { rep : forall (g : graph) (x : A) (p : mtype), Prop }.
 
-
 (* Starting generation of [Rep] instances! *)
-
-(* (* Possibly useful code: *)
-
-Record TypeCtorInfo :=
-  { type_ctor_kername : kername
-  ; type_ctor_inductive : inductive
-  ; type_ctor_term : term
-  }.
-
-Definition getTypeCtor {kind : Type} (T : kind) : TemplateMonad TypeCtorInfo :=
-  '(env, t) <- tmQuoteRec T ;;
-  match t with
-  | tInd ind _ =>
-    let first_kn := inductive_mind ind in
-    match lookup first_kn env with
-    | Some (InductiveDecl mut) =>
-      match nth_error (ind_bodies mut) (inductive_ind ind) with
-      | None =>
-        tmFail ("Could not find #" ++ string_of_nat (inductive_ind ind)
-                ++ " in the mutual type block of " ++ string_of_kername first_kn)
-               (* this should never happen *)
-      | Some one =>
-        ret {| type_ctor_kername := (fst first_kn, ind_name one)
-             ; type_ctor_inductive := ind
-             ; type_ctor_term := t
-             |}
-      end
-    | _ =>
-      tmFail ("Could not find the inductive declaration for "
-              ++ string_of_kername first_kn ++ " in the type environment")
-             (* this should never happen *)
-    end
-  | _ =>
-    tmPrint T ;; tmFail "is not an inductive type constructor."
-  end.
-
-MetaCoq Run (getTypeCtor term).
-*)
 
 Definition generate_instance_type
            (ind : inductive)
            (one : one_inductive_body)
-           (replacer : term -> term) : TemplateMonad term :=
+           (replacer : named_term -> named_term) : TemplateMonad term :=
   (* Convert the type of the type to explicitly named representation *)
   ty <- DB.undeBruijn [] (ind_type one) ;;
   (* Goes over a nested π-type and collects binder names,
      makes up a name where there isn't one.
      It also builds a function to replace the part after the π-binders. *)
   let fix collect
-          (t : term) (count : nat) (replacer : term -> term)
-          : list ident * (term -> term) :=
+          (t : named_term) (count : nat) (replacer : named_term -> named_term)
+          : list ident * (named_term -> named_term) :=
     match t with
     | tProd nAnon ty rest =>
         let '(idents, f) := collect rest (S count) replacer in
@@ -215,55 +199,100 @@ Fixpoint find_missing_instances
     | nil => ret nil
     end.
 
-
-
-
 Record arg_info : Type :=
   { arg_name : BasicAst.ident
-    (* the bound name used in the constructor, inside the pattern *)
+    (* the bound name used in the constructor, inside the pattern in the match *)
   ; p_name : BasicAst.ident
-    (* the bound name used in the exists *)
-  ; arg_type : term
-    (* the term for the main inductive type used *)
+    (* the bound name used in the exists, for the [mtype] *)
+  ; arg_type : dissected_type
+    (* the fully applied type used as an argument *)
     (* TODO think about the fully applied type for polymorphic/dependent types *)
   ; arg_inductive : inductive
-    (* the name of the type constructor used in the argument, like [nat], [list], [option] *)
+    (* the name of the type constructor used in the argument,
+       like [nat], [list], [option] *)
+  ; arg_one : one_inductive_body
+    (* the single definition of the type used in the argument *)
   }.
+
+
+Definition get_ty_info_from_inductive
+           (ind : inductive) : TemplateMonad ty_info :=
+  mut <- tmQuoteInductive (inductive_mind ind) ;;
+  match nth_error (ind_bodies mut) (inductive_ind ind) with
+  | None => tmFail "Wrong index for the mutual inductive block"
+  | Some one =>
+      params <- monad_map (fun c => match decl_name c with
+                           | nAnon => tmFail "Unnamed inductive type parameter"
+                           | nNamed n => ret n
+                           end) (ind_params mut) ;;
+      ret {| ty_name := inductive_mind ind
+           ; ty_body := one
+           ; ty_inductive := ind
+           ; ty_params := params
+           |}
+  end.
+
+(* Get the [ty_info] for the first type in the mutual block. *)
+Definition get_ty_info
+           (kn : kername) : TemplateMonad ty_info :=
+  get_ty_info_from_inductive {| inductive_mind := kn ; inductive_ind := 0 |}.
+
+Definition get_one_from_inductive
+           (ind : inductive) : TemplateMonad one_inductive_body :=
+  ty_body <$> get_ty_info_from_inductive ind.
+
 
 Fixpoint handle_dissected_args
          (args : list dissected_type)
          (count : nat)
-          : TemplateMonad (list arg_info) :=
+         : TemplateMonad (list arg_info) :=
     match args with
     | nil => ret nil
-    | cons (dInd ind) args' =>
+    | cons (dInd ind as spine) args' =>
       rest <- handle_dissected_args args' (S count) ;;
       let arg_s : BasicAst.ident := ("$arg" ++ string_of_nat count)%string in
       let ex_s : BasicAst.ident := ("$p" ++ string_of_nat count)%string in
       let t : term := tInd ind nil in
+      one <- get_one_from_inductive ind ;;
       ret ({| arg_name := arg_s
             ; p_name := ex_s
-            ; arg_type := t
-            ; arg_inductive := ind |} :: rest)
+            ; arg_type := spine
+            ; arg_inductive := ind
+            ; arg_one := one |} :: rest)
+    | cons (dApp (dInd ind) diss as spine) args' =>
+      (* tmFail "Dissected type is an application" ;; *)
+      rest <- handle_dissected_args args' (S count) ;;
+      let arg_s : BasicAst.ident := ("$arg" ++ string_of_nat count)%string in
+      let ex_s : BasicAst.ident := ("$p" ++ string_of_nat count)%string in
+      let t : term := tInd ind nil in
+      one <- get_one_from_inductive ind ;;
+      ret ({| arg_name := arg_s
+            ; p_name := ex_s
+            ; arg_type := spine
+            ; arg_inductive := ind
+            ; arg_one := one |} :: rest)
     | cons decl _ =>
-      tmPrint decl ;;
-      tmFail "Dissected type is not a type"
+      (* tmPrint decl ;; *)
+      tmFail ("Dissected type is not a type" ++ string_of_nat count)
     end.
+
+Definition make_tInd (ind : inductive) : global_term :=
+  tInd ind [].
 
 Fixpoint make_lambdas
          (args : list arg_info)
-         : term -> term :=
+         : named_term -> named_term :=
   match args with
   | nil => fun x => x
   | arg :: args' =>
     fun x => tLambda (nNamed (arg_name arg))
-                     (arg_type arg)
+                     (make_tInd (arg_inductive arg))
                      (make_lambdas args' x)
   end.
 
 Fixpoint make_exists
          (args : list arg_info)
-         : term -> term :=
+         : named_term -> named_term :=
   match args with
   | nil => fun x => x
   | arg :: args' =>
@@ -275,25 +304,39 @@ Fixpoint make_exists
   end.
 
 
-Definition t_cons (t : term) (t' : term) : term :=
+(* Special helper functions to make lists consisting of [mtype] values *)
+Definition t_cons (t : any_term) (t' : any_term) : any_term :=
   tApp <% @cons %> [<% mtype %> ; t ; t'].
-Definition t_conses (xs : list term) : term :=
+Definition t_conses (xs : list any_term) : any_term :=
   fold_right t_cons <% @nil mtype %> xs.
-Definition t_and (t : term) (t' : term) : term :=
+Definition t_and (t : any_term) (t' : any_term) : any_term :=
   tApp <% @and %> [t ; t'].
 
-Print one_inductive_body.
-Compute (seq 0 4).
+(* [tmInferInstance] can create some type checking error
+   but this definition solves it for some reason. *)
+Definition tmInferInstanceEval (t : Type) := tmInferInstance (Some all) t.
+
+(* Takes in a term representing a type like [forall A, Rep (list A)])
+
+*)
+Definition instance_term (inst_ty : term) : TemplateMonad global_term :=
+  inst_ty' <- tmUnquoteTyped Type inst_ty ;;
+  opt_ins <- tmInferInstanceEval inst_ty' ;;
+  match opt_ins with
+  | my_Some x => tmQuote x
+  | _ => tmFail "No such instance"
+  end.
+
 Fixpoint make_prop
          (ind : inductive)
          (one : one_inductive_body)
          (ctor : ctor_info)
          (args : list arg_info)
-         : TemplateMonad term :=
+         : TemplateMonad named_term :=
   let t_g := tVar "$g" in
   let t_p := tVar "$p" in
 
-  let make_prop_base : TemplateMonad term :=
+  let make_prop_base : TemplateMonad named_term :=
     (* Create the [cRep] for this constructor and evaluate *)
     crep <- tmEval all
               (match ctor_arity ctor with
@@ -308,35 +351,34 @@ Fixpoint make_prop
               [ t_g ; t_p ; t_crep ; l])
   in
 
-  (* Takes in the order of the argument and the [arg_info], *)
-(*      generates the call to [rep] for that argument *)
-  let make_arg_prop (arg' : nat * arg_info) : TemplateMonad term :=
+  (* Takes in the order of the argument and the [arg_info],
+     generates the call to [rep] for that argument *)
+  let make_arg_prop (arg' : nat * arg_info) : TemplateMonad named_term :=
     let '(i, arg) := arg' in
     let t_arg := tVar ("$arg" ++ string_of_nat i) in
     let t_p := tVar ("$p" ++ string_of_nat i) in
 
-    (* Check if this is a recursive call to the [rep] we're defining *)
-    if eq_inductive ind (arg_inductive arg)
+    (* Check if this is a recursive call to the [rep] block we're defining *)
+    if eq_kername (inductive_mind ind) (inductive_mind (arg_inductive arg))
     then
-      let t_rep := tVar ("$rep_" ++ ind_name one) in
+      let t_rep :=
+        tVar ("$rep" ++ string_of_nat (inductive_ind (arg_inductive arg))) in
       ret (tApp t_rep [ t_g ; t_arg; t_p ])
     else
       (* not a recursive call, find the right [Rep] instance *)
-      ty <- tmUnquoteTyped Type (arg_type arg) ;;
-      opt_ins <- tmInferInstance (Some all) (Rep ty) ;; (* FIXME polymorphic *)
-      match opt_ins with
-      | my_Some ins =>
-        t_ins <- tmQuote ins ;;
-        ret (tApp <% @rep %> [ arg_type arg ; t_ins ; t_g ; t_arg; t_p ])
-      | my_None =>
-          tmFail ("No instance found")
-      end
+      inst_ty <- generate_instance_type ind one
+                                        (fun t => tApp <% Rep %> [t]) ;;
+      (* TODO fix this for special [Rep] instances *)
+      t_ins <- instance_term inst_ty ;;
+      ret (tApp <% @rep %> [ make_tInd (arg_inductive arg)
+                           ; t_ins ; t_g ; t_arg; t_p ])
   in
   arg_props <- monad_map make_arg_prop (enumerate_nat args) ;;
   base <- make_prop_base ;;
   ret (fold_right t_and base arg_props).
 
-
+(* Takes in the info for a single constructor of a type, generates the branches
+   of a match expression for that constructor. *)
 Definition ctor_to_branch
     (ind : inductive)
       (* the type we're generating for *)
@@ -346,10 +388,16 @@ Definition ctor_to_branch
       (* reified term of the type we're generating for *)
     (ctor : ctor_info)
       (* a single constructor to generate for *)
-    : TemplateMonad (nat * term) :=
+    : TemplateMonad (nat * named_term) :=
+  let kn : kername := inductive_mind ind in
+  mut <- tmQuoteInductive kn ;;
+  let ctx : list dissected_type :=
+      mapi (fun i _ => dInd {| inductive_mind := kn ; inductive_ind := i |})
+           (ind_bodies mut) in
+  params <- ty_params <$> get_ty_info (inductive_mind ind) ;;
   let '(dissected_args, dissected_res) :=
-      (* FIXME params *)
-      dissect_types nil (dInd ind :: nil) (ctor_type ctor) in
+      dissect_types params ctx (ctor_type ctor) in
+  (* tmPrint (dissected_args, dissected_res) ;; *)
   args <- handle_dissected_args dissected_args O ;;
   prop <- make_prop ind one ctor args ;;
   let t := make_lambdas args (make_exists args prop) in
@@ -365,7 +413,7 @@ Definition matchmaker
       (* reified term of the type we're generating for *)
     (ctors : list ctor_info)
       (* constructors we're generating match branches for *)
-    : TemplateMonad term :=
+    : TemplateMonad named_term :=
   branches <- monad_map (ctor_to_branch ind one tau) ctors ;;
   ret (tCase (ind, 0)
              (tLambda (nNamed "$y"%string) tau <% Prop %>)
@@ -379,8 +427,8 @@ Definition matchmaker
 Definition make_fix_single
            (tau : term) (* fully applied type constructor *)
            (ind : inductive)
-           (one : one_inductive_body) : TemplateMonad (BasicAst.def term) :=
-  let this_name := nNamed ("$rep_" ++ ind_name one)%string in
+           (one : one_inductive_body) : TemplateMonad (BasicAst.def named_term) :=
+  let this_name := nNamed ("$rep" ++ string_of_nat (inductive_ind ind)) in
   prop <- matchmaker ind one tau (process_ctors (ind_ctors one)) ;;
   let body :=
       (tLambda (nNamed "$g"%string) <% graph %>
@@ -398,26 +446,26 @@ Definition make_fix_single
        ; rarg := 1 |}.
 
 (* Remove all the initial consecutive π-type quantifiers from a [term]. *)
-Fixpoint strip_quantifiers (t : term) : term :=
+Fixpoint strip_quantifiers (t : named_term) : named_term :=
   match t with
   | tProd _ _ rest => strip_quantifiers rest
   | x => x
   end.
 
 (* Get binder names and binding types for all
-   initial consecutive π-type quantifiers in a [term]. *)
-Fixpoint get_quantifiers (t : term) : list (name * term) :=
+   initial consecutive π-type quantifiers in an [any_term]. *)
+Fixpoint get_quantifiers (t : any_term) : list (name * any_term) :=
   match t with
   | tProd n ty rest => (n, ty) :: get_quantifiers rest
   | x => nil
   end.
 
-(* Given binder names and binding types, add binders to the base [term].
+(* Given binder names and binding types, add binders to the base [named_term].
    Can be used to add λs (with [tLambda]) or πs (with [tProd]). *)
 Fixpoint build_quantifiers
-         (binder : name -> term -> term -> term)
-         (l : list (name * term))
-         (base : term) : term :=
+         (binder : name -> named_term -> named_term -> named_term)
+         (l : list (name * named_term))
+         (base : named_term) : named_term :=
   match l with
   | nil => base
   | (n, t) :: rest => binder n t (build_quantifiers binder rest base)
@@ -459,21 +507,20 @@ Definition add_instances (kn : kername) : TemplateMonad unit :=
                                         <% mtype %>
                                         <% Prop %>)) in
        let quantifiers := get_quantifiers quantified_named in
-       let prog_named : term :=
+       let prog_named : named_term :=
            build_quantifiers tLambda quantifiers
-                             (tApp (tConstruct {| inductive_mind := <? Rep ?>
-                                                ; inductive_ind := 0 |} 0 [])
+                             (tApp <% @Build_Rep %>
                                    [tau; tFix singles i]) in
+       (* tmEval all prog_named >>= tmPrint ;; *)
 
        (* Convert generated program from named to de Bruijn representation *)
        prog <- DB.deBruijn prog_named ;;
 
        (* If need be, here's the reified type of our [Rep] instance: *)
-       (*    instance_ty <-
-               tmUnquoteTyped Type
-                 (build_quantifiers tProd quantifiers
-                                   (tApp <% Rep %> [quantified])) ;;
-       *)
+        instance_ty <-
+              tmUnquoteTyped Type
+                (build_quantifiers tProd quantifiers
+                                  (tApp <% Rep %> [quantified])) ;;
 
        instance <- tmUnquote prog ;;
        (* Remove [tmEval] when MetaCoq issue 455 is fixed: *)
@@ -512,15 +559,106 @@ Definition rep_gen {kind : Type} (Tau : kind) : TemplateMonad unit :=
   monad_iter add_instances (rev missing).
 
 
-(* Let's see it in action: *)
 
-MetaCoq Run (rep_gen bool).
-Print Rep_bool.
+(* Playground: *)
+
+
+(* Instance Rep_nat : Rep nat := *)
+(*   {| rep _ _ _ := False |}. *)
+(* Instance Rep_list {A} `{Rep A} : Rep (list A) := *)
+(*   {| rep _ _ _ := False |}. *)
+
+(* Check <% forall A `{Rep A}, Rep (list A)%>. *)
+(* Check <% forall A, Rep A -> Rep (list A)%>. *)
+(* MetaCoq Run (o <- tmInferInstance (Some all) (forall A, Rep A -> Rep (list A)) ;; *)
+(*              tmPrint o). *)
+
+
+
+
+Check <%% le %%>.
+(* Let's see it in action: *)
+MetaCoq Run (rep_gen unit).
+Print Rep_unit.
+(* fitting_index g p (enum 0) [] *)
+
+(* MetaCoq Run (rep_gen bool). *)
+(* Print Rep_bool. *)
+
+Print name.
+Check <%% list %%>.
+
+Inductive T (n : nat) (eq : n = 0) : nat -> Type :=
+| C : T n eq (n + n).
+
+Instance Rep_T n eq n' : Rep (T n eq n') :=
+  {| rep g x p :=
+       match x with
+       | C => False
+       end
+  |}.
+
+Check <%% T %%>.
+Check (fun (t : T 0 (eq_refl 0) 0) => match t with C => true end).
+
+Fixpoint rep0 (g : graph) (x : nat) (p : mtype) {struct x} : Prop :=
+  match x with
+  | 0 => fitting_index g p (enum 0) []
+  | S arg0 =>
+      exists p0 : mtype, rep0 g arg0 p0 /\ fitting_index g p (boxed 0 1) [p0]
+  end.
+(* Instance Rep_nat : Rep nat := @Build_Rep nat rep0. *)
 
 MetaCoq Run (rep_gen nat).
 Print Rep_nat.
 
-(* MetaCoq Run (rep_gen list). *)
+Inductive vec (A : Type) : nat -> Type :=
+| vnil : vec A O
+| vcons : forall n, A -> vec A n -> vec A (S n).
+
+Instance Rep_vec (A : Type) (Rep_A : Rep A) (n : nat) : Rep (vec A n) :=
+  let fix rep_vec (n : nat) (g : graph) (x : vec A n) (p : mtype) {struct x} : Prop :=
+    match x with
+    | vnil => fitting_index g p (enum 0) []
+    | vcons arg0 arg1 arg2 =>
+        exists p0 p1 p2 : mtype,
+          @rep nat Rep_nat g arg0 p0 /\
+          @rep A Rep_A g arg1 p1 /\
+          rep_vec arg0 g arg2 p2 /\
+          fitting_index g p (boxed 0 3) [p0; p1; p2]
+    end
+  in @Build_Rep (vec A n) (rep_vec n).
+
+Inductive fin : nat -> Set :=
+| F1 : forall {n}, fin (S n)
+| FS : forall {n}, fin n -> fin (S n).
+
+Inductive fin' : Set :=
+| F1' : forall {n : nat}, fin'
+| FS' : forall {n : nat}, fin' -> fin'.
+Check <%% fin %%>.
+
+(* Inductive T (x : unit) : Type := *)
+(* | C : T x. *)
+(* Check <%% T %%>. *)
+MetaCoq Run (rep_gen fin').
+(* Print Rep_fin'. *)
+
+Instance Rep_fin (n : nat) : Rep (fin n) :=
+  let fix rep_fin (n : nat) (g : graph) (x : fin n) (p : mtype) {struct x} : Prop :=
+    match x with
+    | @F1 arg0 =>
+        exists p0 : mtype, rep g arg0 p0 /\ fitting_index g p (boxed 0 1) [p0]
+    | @FS arg0 arg1 =>
+        exists p0 p1 : mtype,
+          rep g arg0 p0 /\
+          rep_fin arg0 g arg1 p1 /\ fitting_index g p (boxed 1 2) [p0; p1]
+    end in @Build_Rep (fin n) (rep_fin n).
+
+MetaCoq Run (rep_gen fin).
+(* Print Rep_fin. *)
+
+MetaCoq Run (rep_gen list).
 (* Print Rep_list. *)
 
 Inductive rgx : Type :=
@@ -531,23 +669,23 @@ Inductive rgx : Type :=
 | and     : rgx -> rgx -> rgx
 | star    : rgx -> rgx.
 
-MetaCoq Run (rep_gen rgx).
-Print Rep_rgx.
+(* MetaCoq Run (rep_gen rgx). *)
+(* Print Rep_rgx. *)
 
 Inductive R1 :=
 | r1 : R1
 with R2 :=
 | r2 : R2.
 
-MetaCoq Run (rep_gen R1).
-Print Rep_R1.
+(* MetaCoq Run (rep_gen R1). *)
+(* Print Rep_R1. *)
 
 Inductive T1 :=
 | c1 : T2 -> T1
 with T2 :=
 | c2 : T1 -> T2.
 
-(* MetaCoq Run (rep_gen T1). *)
+MetaCoq Run (rep_gen T1).
 (* Print Rep_T1. *)
 
 Inductive param_and_index (a b : nat) : a < b -> Type :=
